io/IIO2.fst
@@ -157,7 +157,7 @@ effect IIO
 let static_cmd
   (cmd : io_cmds)
   (arg : io_sig.args cmd) :
-  IIO (io_resm cmd) IOActions
+  IIO (io_sig.res cmd arg) IOActions
     (requires (fun h -> io_pre cmd arg h))
     (ensures (fun h (r:io_sig.res cmd arg) lt ->
         lt == [convert_call_to_event cmd arg r])) =
@@ -178,7 +178,7 @@ let performance_test (#fl:tflag) : IIOwp unit (fl+IOActions) (fun p h -> forall 
   ()
 
 (** ** Model compilation **)
-type rc_typ (t1 t2:Type) = t1 -> trace -> t2 -> trace -> bool
+type rc_typ (t1:Type u#a) (t2:Type u#b) = t1 -> trace -> t2 -> trace -> bool
 
 type eff_rc_typ_cont (fl:erased tflag) (t1:Type u#a) (t2:Type u#b) (rc:rc_typ t1 t2) (x:t1) (initial_h:erased trace) =
   y:t2 -> IIO ((erased trace) * bool) fl (fun h -> (initial_h `suffix_of` h)) (fun h (the_lt, b) lt -> apply_changes initial_h the_lt == h /\ lt == [] /\ (b <==> rc x initial_h y the_lt))
